feat(isomorphism): introduce Coherent inductive type and related theorems for derivations

playground/prototypes/curry-howard/CurryHoward/Isomorphism/Theorems.lean
@@ -56,4 +56,149 @@ namespace CurryHoward.Isomorphism.Theorems
       · exact hA
       · exact ih
 
+  inductive Coherent : Derivation Γ A → (Σ (t : Term), Typing (φ_lift Γ) t (φ A)) → Prop where
+    | hyp
+      (Γ : Context Formula)
+      (i : Fin Γ.length) :
+      Coherent (.hyp i) (extract (.hyp i))
+
+    | implI
+      (Γ : Context Formula)
+      (A B : Formula)
+      (d : Derivation (A :: Γ) B)
+      (jp : Σ (t : Term), Typing (φ_lift (A :: Γ)) t (φ B)) :
+        Coherent d jp →
+        Coherent (.implI A B d) ⟨Term.lam (φ A) jp.1, .lam (φ A) (φ B) jp.1 (ctx_extend_eq A Γ ▸ jp.2)⟩
+
+    | implE
+      (Γ : Context Formula)
+      (A B : Formula)
+      (d₁ : Derivation Γ (Formula.impl A B))
+      (d₂ : Derivation Γ A)
+      (jt₁ jt₂) :
+        Coherent d₁ jt₁ →
+        Coherent d₂ jt₂ →
+        Coherent (.implE A B d₁ d₂) ⟨Term.app jt₁.1 jt₂.1, .app jt₁.1 jt₂.1 (φ A) (φ B) jt₁.2 jt₂.2⟩
+
+    | andI
+      (Γ : Context Formula)
+      (A B : Formula)
+      (d₁ : Derivation Γ A)
+      (d₂ : Derivation Γ B)
+      (jt₁ jt₂) :
+        Coherent d₁ jt₁ →
+        Coherent d₂ jt₂ →
+        Coherent (.andI A B d₁ d₂) ⟨Term.pair jt₁.1 jt₂.1, .pair jt₁.1 jt₂.1 (φ A) (φ B) jt₁.2 jt₂.2⟩
+
+    | andE1
+      (Γ : Context Formula)
+      (A B : Formula)
+      (d : Derivation Γ (Formula.and A B)) (jt) :
+        Coherent d jt →
+        Coherent (.andE1 A B d) ⟨Term.fst jt.1, .fst jt.1 (φ A) (φ B) jt.2⟩
+
+    | andE2
+      (Γ : Context Formula)
+      (A B : Formula)
+      (d : Derivation Γ (Formula.and A B)) (jt) :
+        Coherent d jt →
+        Coherent (.andE2 A B d) ⟨Term.snd jt.1, Typing.snd jt.1 (φ A) (φ B) jt.2⟩
+
+    | orI1 (Γ : Context Formula) (A B : Formula) (d : Derivation Γ A) (jt) :
+        Coherent d jt →
+        Coherent (.orI1 A B d) ⟨Term.inl (φ B) jt.1, .inl jt.1 (φ A) (φ B) jt.2⟩
+
+    | orI2 (Γ : Context Formula) (A B : Formula) (d : Derivation Γ B) (jt) :
+        Coherent d jt →
+        Coherent (.orI2 A B d) ⟨Term.inr (φ A) jt.1, .inr jt.1 (φ A) (φ B) jt.2⟩
+
+    | orE
+      (Γ : Context Formula)
+      (A B C : Formula)
+      (d₀ : Derivation Γ (Formula.or A B))
+      (d₁ : Derivation (A :: Γ) C)
+      (d₂ : Derivation (B :: Γ) C) :
+        Coherent d₀ (extract d₀) →
+        Coherent d₁ (extract d₁) →
+        Coherent d₂ (extract d₂) →
+        Coherent (.orE A B C d₀ d₁ d₂) (extract (.orE A B C d₀ d₁ d₂))
+
+    | topI (Γ : Context Formula) :
+        Coherent .topI ⟨Term.unit, .unit⟩
+
+    | botE
+      (Γ : Context Formula)
+      (A : Formula)
+      (d : Derivation Γ .bot) :
+        Coherent d (extract d) →
+        Coherent (.botE A d) (extract (.botE A d))
+
+  theorem extract_is_coherent {Γ : Context Formula} {A : Formula}
+    (d : Derivation Γ A) :  Coherent d (extract d) := by
+    induction d with
+    | hyp i =>
+      rename_i Γ_locale
+      dsimp [extract]
+      exact .hyp Γ_locale i
+
+    | implI A B d ih =>
+      rename_i Γ_locale
+      dsimp [extract]
+      exact .implI Γ_locale A B d (extract d) ih
+
+    | implE A B d₁ d₂ ih₁ ih₂ =>
+      rename_i Γ_locale
+      dsimp [extract]
+      exact .implE Γ_locale A B d₁ d₂ (extract d₁) (extract d₂) ih₁ ih₂
+
+    | andI A B d₁ d₂ ih₁ ih₂ =>
+      rename_i Γ_locale
+      dsimp [extract]
+      exact .andI Γ_locale A B d₁ d₂ (extract d₁) (extract d₂) ih₁ ih₂
+
+    | andE1 A B d ih =>
+      rename_i Γ_locale
+      dsimp [extract]
+      exact .andE1 Γ_locale A B d (extract d) ih
+
+    | andE2 A B d ih =>
+      rename_i Γ_locale
+      dsimp [extract]
+      exact .andE2 Γ_locale A B d (extract d) ih
+
+    | orI1 A B d ih =>
+      rename_i Γ_locale
+      dsimp [extract]
+      exact .orI1 Γ_locale A B d (extract d) ih
+
+    | orI2 A B d ih =>
+      rename_i Γ_locale
+      dsimp [extract]
+      exact .orI2 Γ_locale A B d (extract d) ih
+
+    |  orE A B C d₀ d₁ d₂ ih₀ ih₁ ih₂ =>
+      rename_i Γ_locale
+      exact .orE Γ_locale A B C d₀ d₁ d₂ ih₀ ih₁ ih₂
+
+    | topI =>
+      rename_i Γ_locale
+      dsimp [extract]
+      exact .topI Γ_locale
+
+    | botE A d ih =>
+      rename_i Γ_locale
+      exact .botE Γ_locale A d ih
+
+  theorem embed_is_coherent {Γ : Context Formula} {A : Formula} {t : Term}
+    (jt : Typing (φ_lift Γ) t (φ A)) :
+    Coherent (
+      have h_ctx : iφ_lift (φ_lift Γ) = Γ := by
+        change (iφ_lift ∘ φ_lift) Γ = id Γ
+        rw [iφ_lift_φ_lift_eq]
+      have h_type : iφ (φ A) = A := by
+        change (iφ ∘ φ) A = id A
+        rw [iφ_φ_eq]
+      h_ctx ▸ h_type ▸ (embed jt)
+    ) ⟨t, jt⟩ := by sorry
+
 end CurryHoward.Isomorphism.Theorems
